qed wp for evidServLink__check

src/program_proof/pav/evidence.v
@@ -14,19 +14,23 @@ Record t :=
   }.
 
 Definition encodesF (obj : t) : list w8 :=
-  [(W8 1)] ++ u64_le obj.(epoch) ++ obj.(prevLink) ++ obj.(data).
+  [(W8 1)] ++ u64_le obj.(epoch) ++ u64_le (length obj.(prevLink)) ++ obj.(prevLink) ++ u64_le (length obj.(data)) ++ obj.(data).
 Definition encodes (enc : list w8) (obj : t) : Prop :=
   enc = encodesF obj.
+
+Lemma inj obj0 obj1 :
+  encodesF obj0 = encodesF obj1 → obj0 = obj1.
+Proof. Admitted.
 
 Section local_defs.
 Context `{!heapGS Σ}.
 Definition own ptr obj : iProp Σ :=
-  ∃ sl_prevLink sl_data,
+  ∃ sl_prevLink sl_data d0 d1,
   "Hepoch" ∷ ptr ↦[chainSepSome :: "epoch"] #obj.(epoch) ∗
   "HprevLink" ∷ ptr ↦[chainSepSome :: "prevLink"] (slice_val sl_prevLink) ∗
-  "Hsl_prevLink" ∷ own_slice_small sl_prevLink byteT (DfracOwn 1) obj.(prevLink) ∗
+  "Hsl_prevLink" ∷ own_slice_small sl_prevLink byteT d0 obj.(prevLink) ∗
   "Hdata" ∷ ptr ↦[chainSepSome :: "data"] (slice_val sl_data) ∗
-  "Hsl_data" ∷ own_slice_small sl_data byteT (DfracOwn 1) obj.(data).
+  "Hsl_data" ∷ own_slice_small sl_data byteT d1 obj.(data).
 
 Lemma wp_encode ptr obj :
   {{{
@@ -50,16 +54,20 @@ Record t :=
   }.
 
 Definition encodesF (obj : t) : list w8 :=
-  [(W8 0)] ++ obj.(link).
+  [(W8 0)] ++ u64_le (length obj.(link)) ++ obj.(link).
 Definition encodes (enc : list w8) (obj : t) : Prop :=
   enc = encodesF obj.
+
+Lemma inj obj0 obj1 :
+  encodesF obj0 = encodesF obj1 → obj0 = obj1.
+Proof. Admitted.
 
 Section local_defs.
 Context `{!heapGS Σ}.
 Definition own ptr obj : iProp Σ :=
-  ∃ sl_link,
+  ∃ sl_link d0,
   "Hlink" ∷ ptr ↦[servSepLink :: "link"] (slice_val sl_link) ∗
-  "Hsl_link" ∷ own_slice_small sl_link byteT (DfracOwn 1) obj.(link).
+  "Hsl_link" ∷ own_slice_small sl_link byteT d0 obj.(link).
 
 Lemma wp_encode ptr obj :
   {{{
@@ -85,7 +93,7 @@ Record t :=
   }.
 
 Definition encodesF (obj : t) : list w8 :=
-  [(W8 1)] ++ u64_le obj.(epoch) ++ obj.(id) ++ obj.(val).
+  [(W8 1)] ++ u64_le obj.(epoch) ++ u64_le (length obj.(id)) ++ obj.(id) ++ u64_le (length obj.(val)) ++ obj.(val).
 Definition encodes (enc : list w8) (obj : t) : Prop :=
   enc = encodesF obj.
 End servSepPut.
@@ -107,33 +115,46 @@ Record t :=
 Section local_defs.
 Context `{!heapGS Σ}.
 Definition own ptr obj : iProp Σ :=
-  ∃ sl_prevLink0 sl_dig0 sl_sig0 sl_prevLink1 sl_dig1 sl_sig1,
+  ∃ sl_prevLink0 sl_dig0 sl_sig0 sl_prevLink1 sl_dig1 sl_sig1 d0 d1 d2 d3 d4 d5,
   "Hepoch0" ∷ ptr ↦[evidServLink :: "epoch0"] #obj.(epoch0) ∗
   "HprevLink0" ∷ ptr ↦[evidServLink :: "prevLink0"] (slice_val sl_prevLink0) ∗
-  "Hsl_prevLink0" ∷ own_slice_small sl_prevLink0 byteT (DfracOwn 1) obj.(prevLink0) ∗
+  "Hsl_prevLink0" ∷ own_slice_small sl_prevLink0 byteT d0 obj.(prevLink0) ∗
   "Hdig0" ∷ ptr ↦[evidServLink :: "dig0"] (slice_val sl_dig0) ∗
-  "Hsl_dig0" ∷ own_slice_small sl_dig0 byteT (DfracOwn 1) obj.(dig0) ∗
+  "Hsl_dig0" ∷ own_slice_small sl_dig0 byteT d1 obj.(dig0) ∗
   "Hsig0" ∷ ptr ↦[evidServLink :: "sig0"] (slice_val sl_sig0) ∗
-  "Hsl_sig0" ∷ own_slice_small sl_sig0 byteT (DfracOwn 1) obj.(sig0) ∗
+  "Hsl_sig0" ∷ own_slice_small sl_sig0 byteT d2 obj.(sig0) ∗
 
   "Hepoch1" ∷ ptr ↦[evidServLink :: "epoch1"] #obj.(epoch1) ∗
   "HprevLink1" ∷ ptr ↦[evidServLink :: "prevLink1"] (slice_val sl_prevLink1) ∗
-  "Hsl_prevLink1" ∷ own_slice_small sl_prevLink1 byteT (DfracOwn 1) obj.(prevLink1) ∗
+  "Hsl_prevLink1" ∷ own_slice_small sl_prevLink1 byteT d3 obj.(prevLink1) ∗
   "Hdig1" ∷ ptr ↦[evidServLink :: "dig1"] (slice_val sl_dig1) ∗
-  "Hsl_dig1" ∷ own_slice_small sl_dig1 byteT (DfracOwn 1) obj.(dig1) ∗
+  "Hsl_dig1" ∷ own_slice_small sl_dig1 byteT d4 obj.(dig1) ∗
   "Hsig1" ∷ ptr ↦[evidServLink :: "sig1"] (slice_val sl_sig1) ∗
-  "Hsl_sig1" ∷ own_slice_small sl_sig1 byteT (DfracOwn 1) obj.(sig1).
+  "Hsl_sig1" ∷ own_slice_small sl_sig1 byteT d5 obj.(sig1).
 End local_defs.
 End evidServLink.
 
 Section evidence.
 Context `{!heapGS Σ, !mono_listG (list w8) Σ}.
 
+(* Note: the more general version of this lemma has a set of encodings
+   that are within the same domain.
+   if any two of these hold, we can prove false.
+   there'd need to be a side req that each encoding has a diff tag. *)
+Lemma servSep enc obj0 obj1 :
+  servSepLink.encodes enc obj0 ∧ servSepPut.encodes enc obj1 → False.
+Proof.
+  intros [HencLink HencPut].
+  rewrite /servSepLink.encodes /servSepLink.encodesF in HencLink.
+  rewrite /servSepPut.encodes /servSepPut.encodesF in HencPut.
+  naive_solver.
+Qed.
+
 Definition serv_sigpred_link γ (data : servSepLink.t) : iProp Σ :=
   ∃ (links : list (list w8)) (epoch : w64) (prevLink : list w8) (currDig : list w8),
   "#Hlinks" ∷ mono_list_lb_own γ links ∗
-  "#Hlink" ∷ is_hash data.(servSepLink.link) (chainSepSome.encodesF (chainSepSome.mk epoch prevLink currDig)) ∗
-  "%HlookPrev" ∷ ⌜links !! (uint.nat epoch - 1) = Some prevLink⌝ ∗
+  "#Hlink" ∷ is_hash (chainSepSome.encodesF (chainSepSome.mk epoch prevLink currDig)) data.(servSepLink.link) ∗
+  "%HlookPrev" ∷ ⌜links !! (uint.nat (word.sub epoch (W64 1))) = Some prevLink⌝ ∗
   "%HlookCurr" ∷ ⌜links !! uint.nat epoch = Some data.(servSepLink.link)⌝.
 
 (* Note: False for now so we don't have to consider put promises. *)
@@ -161,7 +182,6 @@ Lemma wp_evidServLink_check ptr_evid evid pk γ hon :
   evidServLink__check #ptr_evid (slice_val pk)
   {{{
     (err : bool), RET #err;
-    "Hevid" ∷ evidServLink.own ptr_evid evid ∗
     if negb err then
       "%Hhon" ∷ ⌜hon = false⌝
     else True%I
@@ -170,6 +190,8 @@ Proof.
   rewrite /evidServLink__check.
   iIntros (Φ) "H HΦ"; iNamed "H".
   iDestruct "Hevid" as (??????) "H"; iNamed "H".
+
+  (* first link sig. *)
   wp_loadField.
   wp_loadField.
   wp_loadField.
@@ -177,11 +199,12 @@ Proof.
     iIntros (ptr_linkSep0) "Hptr_linkSep0".
   iDestruct (struct_fields_split with "Hptr_linkSep0") as "H";
     iNamed "H"; iClear "tag".
+  iMod (own_slice_small_persist with "Hsl_prevLink0") as "#Hsl_prevLink0".
   wp_apply (chainSepSome.wp_encode with "[epoch prevLink data Hsl_prevLink0 Hsl_dig0]").
   {
     instantiate (1:=chainSepSome.mk _ _ _).
     rewrite /chainSepSome.own /=.
-    iExists sl_prevLink0; iFrame.
+    iExists sl_prevLink0, sl_dig0; iFrame "#∗".
   }
   iIntros (sl_link0Enc link0Enc) "H"; iNamed "H";
     iRename "Hobj" into "Hptr_linkSep0";
@@ -192,15 +215,16 @@ Proof.
     iRename "Hdata" into "Hsl_link0Enc";
     iRename "Hhash" into "Hsl_link0";
     iRename "His_hash" into "His_hash_link0".
+  iMod (own_slice_small_persist with "Hsl_link0") as "#Hsl_link0".
   wp_apply wp_allocStruct; [val_ty|];
     iIntros (ptr_enc0) "Hptr_enc0".
   iDestruct (struct_fields_split with "Hptr_enc0") as "H";
     iNamed "H"; iClear "tag".
-  wp_apply (servSepLink.wp_encode with "[link Hsl_link0]").
+  wp_apply (servSepLink.wp_encode with "[link]").
   {
     instantiate (1:=servSepLink.mk _).
     rewrite /servSepLink.own /=.
-    iFrame.
+    iFrame "#∗".
   }
   iIntros (sl_enc0 enc0) "H"; iNamed "H";
     iRename "Hobj" into "Hptr_enc0";
@@ -210,7 +234,140 @@ Proof.
   wp_apply (wp_Verify with "[Hsl_enc0 Hsl_sig0]"); [iFrame "#∗"|];
     iIntros (?) "H"; iNamed "H";
     iRename "Hsig" into "Hsl_sig0";
-    iRename "Hmsg" into "Hsl_enc0".
+    iRename "Hmsg" into "Hsl_enc0";
+    iRename "HP" into "Hsigpred0".
   destruct ok.
-Admitted.
+  2: { wp_pures. by iApply "HΦ". }
+
+  (* second link sig. *)
+  wp_loadField.
+  wp_loadField.
+  wp_loadField.
+  wp_apply wp_allocStruct; [val_ty|];
+    iIntros (ptr_linkSep1) "Hptr_linkSep1".
+  iDestruct (struct_fields_split with "Hptr_linkSep1") as "H";
+    iNamed "H"; iClear "tag".
+  iMod (own_slice_small_persist with "Hsl_prevLink1") as "#Hsl_prevLink1".
+  wp_apply (chainSepSome.wp_encode with "[epoch prevLink data Hsl_prevLink1 Hsl_dig1]").
+  {
+    instantiate (1:=chainSepSome.mk _ _ _).
+    rewrite /chainSepSome.own /=.
+    iExists sl_prevLink1, sl_dig1; iFrame "#∗".
+  }
+  iIntros (sl_link1Enc link1Enc) "H"; iNamed "H";
+    iRename "Hobj" into "Hptr_linkSep1";
+    iRename "Hsl_enc" into "Hsl_link1Enc";
+    rename Henc into Henc_link1.
+  wp_apply (wp_Hash with "Hsl_link1Enc");
+    iIntros (sl_link1 link1) "H"; iNamed "H";
+    iRename "Hdata" into "Hsl_link1Enc";
+    iRename "Hhash" into "Hsl_link1";
+    iRename "His_hash" into "His_hash_link1".
+  iMod (own_slice_small_persist with "Hsl_link1") as "#Hsl_link1".
+  wp_apply wp_allocStruct; [val_ty|];
+    iIntros (ptr_enc1) "Hptr_enc1".
+  iDestruct (struct_fields_split with "Hptr_enc1") as "H";
+    iNamed "H"; iClear "tag".
+  wp_apply (servSepLink.wp_encode with "[link]").
+  {
+    instantiate (1:=servSepLink.mk _).
+    rewrite /servSepLink.own /=.
+    iFrame "#∗".
+  }
+  iIntros (sl_enc1 enc1) "H"; iNamed "H";
+    iRename "Hobj" into "Hptr_enc1";
+    iRename "Hsl_enc" into "Hsl_enc1";
+    rename Henc into Henc_enc1.
+  wp_loadField.
+  wp_apply (wp_Verify with "[Hsl_enc1 Hsl_sig1]"); [iFrame "#∗"|];
+    iIntros (?) "H"; iNamed "H";
+    iRename "Hsig" into "Hsl_sig1";
+    iRename "Hmsg" into "Hsl_enc1".
+    iRename "HP" into "Hsigpred1".
+  destruct ok.
+  2: { wp_pures. by iApply "HΦ". }
+
+  (* epochs are equal. *)
+  wp_loadField.
+  wp_loadField.
+  wp_if_destruct; rename Heqb into Hepoch_eq.
+  1: {
+    (* TODO: why does:
+      wp_apply (wp_BytesEqual "[$Hsl_link0 $Hsl_link1]").
+      not work? *)
+    wp_apply wp_BytesEqual; [iFrame "#"|].
+    iIntros "_".
+    case_bool_decide; [by iApply "HΦ"|]; rename H into Hlink_ne.
+    destruct hon; [|by iApply "HΦ"].
+    iDestruct "Hsigpred0" as "[[%sepLink0 [%Henc_link0' Hsigpred0]] | [% [%Henc_put _]]]".
+    2: { exfalso. eauto using servSep. }
+    iDestruct "Hsigpred1" as "[[%sepLink1 [%Henc_link1' Hsigpred1]] | [% [%Henc_put _]]]".
+    2: { exfalso. eauto using servSep. }
+
+    (* open binding, apply val divergence to prove false. *)
+    iExFalso.
+    rewrite ->Henc_link0' in Henc_enc0;
+      apply servSepLink.inj in Henc_enc0 as ->.
+    rewrite ->Henc_link1' in Henc_enc1;
+      apply servSepLink.inj in Henc_enc1 as ->.
+    iDestruct "Hsigpred0" as (links0 epoch0 prevLink0 currDig0) "H";
+      iNamed "H"; iRename "Hlinks" into "Hlinks0";
+      iRename "Hlink" into "Hlink0";
+      move: {HlookPrev} HlookCurr => HlookCurr0.
+    iDestruct "Hsigpred1" as (links1 epoch1 prevLink1 currDig1) "H";
+      iNamed "H"; iRename "Hlinks" into "Hlinks1";
+      iRename "Hlink" into "Hlink1";
+      move: {HlookPrev} HlookCurr => HlookCurr1.
+    iDestruct (hash_inj with "[$His_hash_link0] [$Hlink0]") as %->.
+    iDestruct (hash_inj with "[$His_hash_link1] [$Hlink1]") as %->.
+    apply chainSepSome.inj in Henc_link0 as [=]; subst.
+    apply chainSepSome.inj in Henc_link1 as [=]; subst.
+    rewrite Hepoch_eq in HlookCurr0.
+    iDestruct (mono_list_idx_own_get with "[$Hlinks0]") as "Hidx0"; [done|].
+    iDestruct (mono_list_idx_own_get with "[$Hlinks1]") as "Hidx1"; [done|].
+    iDestruct (mono_list_idx_agree with "[$Hidx0] [$Hidx1]") as %[=].
+    done.
+  }
+
+  (* epochs are off by one, but apart from that,
+     almost same analysis as epoch equals case. *)
+  wp_loadField.
+  wp_loadField.
+  wp_if_destruct; rename Heqb into Hepoch_off_eq.
+  1: {
+    wp_loadField.
+    wp_apply wp_BytesEqual; [iFrame "#"|].
+    iIntros "_".
+    case_bool_decide; [by iApply "HΦ"|]; rename H into Hlink_ne.
+    destruct hon; [|by iApply "HΦ"].
+    iDestruct "Hsigpred0" as "[[%sepLink0 [%Henc_link0' Hsigpred0]] | [% [%Henc_put _]]]".
+    2: { exfalso. eauto using servSep. }
+    iDestruct "Hsigpred1" as "[[%sepLink1 [%Henc_link1' Hsigpred1]] | [% [%Henc_put _]]]".
+    2: { exfalso. eauto using servSep. }
+
+    iExFalso.
+    rewrite ->Henc_link0' in Henc_enc0;
+      apply servSepLink.inj in Henc_enc0 as ->.
+    rewrite ->Henc_link1' in Henc_enc1;
+      apply servSepLink.inj in Henc_enc1 as ->.
+    iDestruct "Hsigpred0" as (links0 epoch0 prevLink0 currDig0) "H";
+      iNamed "H"; iRename "Hlinks" into "Hlinks0";
+      iRename "Hlink" into "Hlink0";
+      move: {HlookPrev} HlookCurr => HlookCurr0.
+    iDestruct "Hsigpred1" as (links1 epoch1 prevLink1 currDig1) "H";
+      iNamed "H"; iRename "Hlinks" into "Hlinks1";
+      iRename "Hlink" into "Hlink1";
+      move: HlookPrev {HlookCurr} => HlookPrev1.
+    iDestruct (hash_inj with "[$His_hash_link0] [$Hlink0]") as %->.
+    iDestruct (hash_inj with "[$His_hash_link1] [$Hlink1]") as %->.
+    apply chainSepSome.inj in Henc_link0 as [=]; subst.
+    apply chainSepSome.inj in Henc_link1 as [=]; subst.
+    rewrite <- Hepoch_off_eq in HlookPrev1.
+    iDestruct (mono_list_idx_own_get with "[$Hlinks0]") as "Hidx0"; [done|].
+    iDestruct (mono_list_idx_own_get with "[$Hlinks1]") as "Hidx1"; [done|].
+    iDestruct (mono_list_idx_agree with "[$Hidx0] [$Hidx1]") as %[=].
+    done.
+  }
+  by iApply "HΦ".
+Qed.
 End evidence.
